add CoeFun instances

Primus/Core/NatTrans.lean
@@ -3,11 +3,15 @@ import Primus.Core.Functor
 
 @[ext]
 structure NaturalTransformation{CC DD: Cat}(F G: Fun CC DD): Sort _ where
-  η: (A: CC.Ob) -> DD.Hom (F.onOb A) (G.onOb A)
+  η: (A: CC.Ob) -> DD.Hom (F A) (G A)
   naturality{A B: CC.Ob}(f: CC.Hom A B): η B ≪ F.onHom f = G.onHom f ≪ η A
 
+instance {CC DD: Cat} {F G: Fun CC DD} :
+    CoeFun (NaturalTransformation F G) (fun _ => ∀ A : CC.Ob, DD.Hom (F A) (G A)) where
+  coe α := α.η
+
 def natTransId{CC DD: Cat}(F: Fun CC DD): NaturalTransformation F F := {
-  η A := DD.id (F.onOb A),
+  η A := DD.id (F A),
   naturality{A B} f := by
     rw [DD.left_id, DD.right_id]
 }
@@ -15,7 +19,7 @@ def natTransId{CC DD: Cat}(F: Fun CC DD): NaturalTransformation F F := {
 def natTransComp{CC DD: Cat}{F G H: Fun CC DD}
   (ntG: NaturalTransformation G H)
   (ntF: NaturalTransformation F G): NaturalTransformation F H := {
-  η A := ntG.η A ≪ ntF.η A,
+  η A := ntG A ≪ ntF A,
   naturality{A B} f := by
     rw [DD.assoc, ←ntG.naturality f, ←DD.assoc, ntF.naturality f, DD.assoc]
   }
